spc/sProp.v
@@ -38,19 +38,19 @@ End HRA.
 
 Coercion HRA.subG_map: HRA.subG >-> Funclass.
 
-Module gTyp.
+Module GTyp.
 
   Class t: Type := __GTYP : GPF.t.
 
-End gTyp.
+End GTyp.
 
 Module SL.
 
   Section SL.
 
-  Context `{sub: @HRA.subG Γ Σ}.
-  Context `{τ: gTyp.t}.
-    
+  Context `{τ: GTyp.t}.
+  Context `{_C0: @HRA.subG Γ Σ}.
+
   Global Instance domain : SRFDom.t := {
     dom := iProp;
     void := False%I;
@@ -119,31 +119,31 @@ Module SL.
   
   Definition ownm `{IN: @GRA.inG M Γ} {n} (r: M) : SRFSyn.t n.
     destruct IN. subst.
-    refine ⟨ existT (_ownm _ r) _ ⟩%SRF.
+    refine ⟨ _ownm _ r, _ ⟩%SRF.
     i. inv X.
   Defined.
 
   Definition pure {n} (P: Prop) : SRFSyn.t n.
-    refine ⟨ existT (_pure P) _ ⟩%SRF.
+    refine ⟨ _pure P, _ ⟩%SRF.
     i. inv X.
   Defined.
 
   Definition and {n} (p1 p2: SRFSyn.t n) : SRFSyn.t n.
-    refine ⟨ existT (_and) _ ⟩%SRF.
+    refine ⟨ _and, _ ⟩%SRF.
     i. destruct X.
     - exact p1.
     - exact p2.
   Defined.
 
   Definition or {n} (p1 p2: SRFSyn.t n) : SRFSyn.t n.
-    refine ⟨ existT (_or) _ ⟩%SRF.
+    refine ⟨ _or, _ ⟩%SRF.
     i. destruct X.
     - exact p1.
     - exact p2.
   Defined.
 
   Definition impl {n} (p1 p2: SRFSyn.t n) : SRFSyn.t n.
-    refine ⟨ existT (_impl) _ ⟩%SRF.
+    refine ⟨ _impl, _ ⟩%SRF.
     i. destruct X.
     - exact p1.
     - exact p2.
@@ -151,47 +151,47 @@ Module SL.
   
   Definition univ `{IN: @GPF.inG T τ} {n} (ty:T) (p: PF.deg ty (SRFSyn._t n) -> SRFSyn.t n) : SRFSyn.t n.
     destruct IN. subst.
-    exact (⟨ existT (_univ _ ty : syntax.(PF.shp)) p ⟩)%SRF.
+    exact ⟨ _univ _ ty, p ⟩%SRF.
   Defined.
 
   Definition ex `{IN: @GPF.inG T τ} {n} (ty: T) (p: PF.deg ty (SRFSyn._t n) -> SRFSyn.t n) : SRFSyn.t n.
     destruct IN. subst.
-    exact (⟨ existT (_ex _ ty : syntax.(PF.shp)) p ⟩)%SRF.
+    exact ⟨ _ex _ ty, p ⟩%SRF.
   Defined.
 
   Definition empty {n} : SRFSyn.t n.
-    refine ⟨ existT (_empty) _ ⟩%SRF.
+    refine ⟨ _empty, _ ⟩%SRF.
     i. inv X.
   Defined.
   
   Definition sepconj {n} (p1 p2: SRFSyn.t n) : SRFSyn.t n.
-    refine ⟨ existT (_sepconj) _ ⟩%SRF.
+    refine ⟨ _sepconj, _ ⟩%SRF.
     i. destruct X.
     - exact p1.
     - exact p2.
   Defined.
 
   Definition wand {n} (p1 p2: SRFSyn.t n) : SRFSyn.t n.
-    refine ⟨ existT (_wand) _ ⟩%SRF.
+    refine ⟨ _wand, _ ⟩%SRF.
     i. destruct X.
     - exact p1.
     - exact p2.
   Defined.
   
   Definition persistently {n} (p: SRFSyn.t n) : SRFSyn.t n.
-    refine ⟨ existT (_persistently) _ ⟩%SRF.
+    refine ⟨ _persistently, _ ⟩%SRF.
     i. inv X; [|inv H1].
     exact p.
   Defined.
 
   Definition plainly {n} (p: SRFSyn.t n) : SRFSyn.t n.
-    refine ⟨ existT (_plainly) _ ⟩%SRF.
+    refine ⟨ _plainly, _ ⟩%SRF.
     i. inv X; [|inv H1].
     exact p.
   Defined.
 
   Definition upd {n} (p: SRFSyn.t n) : SRFSyn.t n.
-    refine ⟨ existT (_upd) _ ⟩%SRF.
+    refine ⟨ _upd, _ ⟩%SRF.
     i. inv X; [|inv H1].
     exact p.
   Defined.
@@ -207,7 +207,7 @@ Module SLRed.
 
   Section RED.
 
-  Context `{τ: gTyp.t}.
+  Context `{τ: GTyp.t}.
   Context `{@HRA.subG Γ Σ}.
   Context `{@SRFMSemG.inG _ _ α SL.t β}.
   
@@ -374,6 +374,155 @@ Ltac SL_red_unary_all := (try rewrite ! @SLRed.ownm in *;
                          ).
 
 Ltac SL_red_all := repeat (SL_red_binary_all; SL_red_unary_all).
+
+
+
+
+Module BO.
+
+  Section BIGOP.
+
+  Context `{τ: GTyp.t}.
+  Context `{_C0: @HRA.subG Γ Σ}.
+  Context `{_C2: @SRFMSemG.inG _ SL.syntax α (@SL.t τ Γ Σ sub α) β}.
+
+  (* Maybe we can make Syntax as an instance for big_opMs. *)
+  Definition syn_big_sepM
+             n {K} {H1 : EqDecision K} {H2 : Countable K}
+             {A} (I : @gmap K H1 H2 A)
+             (f : K -> A -> SRFSyn.t n)
+    : SRFSyn.t n :=
+    fold_right (fun hd tl => (uncurry f hd) ∗ tl)%SRF SL.empty (map_to_list I).
+
+  Lemma red_syn_big_sepM n K {H1 : EqDecision K} {H2 : Countable K} A I f :
+    SRFSem.t n (@syn_big_sepM n K _ _ A I f) = ([∗ map] i ↦ a ∈ I, SRFSem.t n (f i a))%I.
+  Proof.
+    ss. unfold big_opM. rewrite seal_eq. unfold big_op.big_opM_def.
+    unfold syn_big_sepM. simpl. remember (map_to_list I) as L.
+    clear HeqL I. induction L.
+    { ss. SL_red_all. eauto. }
+    ss. SL_red_all. rewrite IHL. f_equal.
+    destruct a. ss.
+  Qed.
+
+  Definition syn_big_sepS
+             n {K} {H1 : EqDecision K} {H2 : Countable K}
+             (I : @gset K H1 H2)
+             (f : K -> SRFSyn.t n)
+    : SRFSyn.t n :=
+    fold_right (fun hd tl => (f hd) ∗ tl)%SRF emp%SRF (elements I).
+
+  Lemma red_syn_big_sepS n K {H1 : EqDecision K} {H2 : Countable K} I f :
+    SRFSem.t n (@syn_big_sepS n K _ _ I f) = ([∗ set] i ∈ I, SRFSem.t n (f i))%I.
+  Proof.
+    ss. unfold big_opS. rewrite seal_eq. unfold big_op.big_opS_def.
+    unfold syn_big_sepS. remember (elements I) as L.
+    clear HeqL I. induction L.
+    { ss. SL_red_all. eauto. }
+    ss. SL_red_all. rewrite IHL. f_equal.
+  Qed.
+
+  Definition syn_big_sepL1
+             n {A} (I : list A)
+             (f : A -> SRFSyn.t n)
+    : SRFSyn.t n :=
+    fold_right (fun hd tl => (f hd) ∗ tl)%SRF emp%SRF I.
+
+  Lemma red_syn_big_sepL1 n A I f :
+    SRFSem.t n (@syn_big_sepL1 n A I f) = ([∗ list] a ∈ I, SRFSem.t n (f a))%I.
+  Proof.
+    ss. induction I; ss.
+    { SL_red_all. ss. }
+    SL_red_all. rewrite IHI. f_equal.
+  Qed.
+
+  End BIGOP.
+
+End BO.
+  
+(* Notations. *)
+Notation "'[∗' n 'map]' k ↦ x ∈ m , P" :=
+  (BO.syn_big_sepM n m (fun k x => P))
+    (at level 200, n at level 1, m at level 10, k, x at level 1, right associativity,
+      format "[∗  n  map]  k  ↦  x  ∈  m ,  P") : formula_scope.
+Notation "'[∗' n , A 'map]' k ↦ x ∈ m , P" :=
+  (BO.syn_big_sepM n (A:=A) m (fun k x => P))
+    (at level 200, n at level 1, m at level 10, k, x, A at level 1, right associativity,
+      format "[∗  n  ,  A  map]  k  ↦  x  ∈  m ,  P") : formula_scope.
+Notation "'[∗' n 'set]' x ∈ X , P" :=
+  (BO.syn_big_sepS n X (fun x => P))
+    (at level 200, n at level 1, X at level 10, x at level 1, right associativity,
+      format "[∗  n  set]  x  ∈  X ,  P") : formula_scope.
+Notation "'[∗' n 'list]' x ∈ l , P" :=
+  (BO.syn_big_sepL1 n l (fun x => P))
+    (at level 200, n at level 1, l at level 10, x at level 1, right associativity,
+      format "[∗  n  list]  x  ∈  l ,  P") : formula_scope.
+Notation "'[∗' n , A 'list]' x ∈ l , P" :=
+  (BO.syn_big_sepL1 n (A:=A) l (fun x => P))
+    (at level 200, n at level 1, l at level 10, x, A at level 1, right associativity,
+      format "[∗  n ,  A  list]  x  ∈  l ,  P") : formula_scope.
+
+
+(** Types of TL. *)
+
+Module ST.
+
+  Section TYPES.
+
+  Inductive type : Type :=
+  | baseT (t : Type) : type
+  | sPropT : type
+  | funT : type -> type -> type
+  | prodT : type -> type -> type
+  | sumT : type -> type -> type
+  | listT : type -> type
+  | pgmapT : type -> type
+  | metaT : type
+  .
+
+  Fixpoint interp (ty : type) (sProp : Type) : Type :=
+    match ty with
+    | baseT b => b
+    | sPropT => sProp
+    | funT ty1 ty2 => (interp ty1 sProp -> interp ty2 sProp)
+    | prodT ty1 ty2 => prod (interp ty1 sProp) (interp ty2 sProp)
+    | sumT ty1 ty2 => sum (interp ty1 sProp) (interp ty2 sProp)
+    | listT ty1 => list (interp ty1 sProp)
+    | pgmapT ty1 => gmap positive (interp ty1 sProp)
+    | metaT => Type
+    end.
+
+  Global Instance t : PF.t := {
+      shp := type;
+      deg := interp;
+    }.
+  
+  End TYPES.
+  
+End ST.
+
+(** Notations and Coercions. *)
+Coercion ST.baseT : Sortclass >-> ST.type.
+
+Declare Scope formula_type_scope.
+Delimit Scope formula_type_scope with ftype.
+Bind Scope formula_type_scope with ST.type.
+
+Notation "⇣ T" := (ST.baseT T) (at level 90) : formula_type_scope.
+Notation "'Φ'" := (ST.sPropT) : formula_type_scope.
+Infix "->" := (ST.funT) : formula_type_scope.
+Infix "*" := (ST.prodT) : formula_type_scope.
+Infix "+" := (ST.sumT) : formula_type_scope.
+
+(** Notations and coercions. *)
+Notation "'τ{' t ',' n '}'" := (PF.deg t (SRFSyn._t n)) : formula_type_scope.
+Notation "'τ{' t '}'" := (PF.deg t (SRFSyn._t _)) : formula_type_scope.
+
+
+
+
+
+
 
 (* Module TestLock. *)
   
